src/lib/poly/gemm/Kuiper.Poly.GEMM.TensorCore2D.fsti
@@ -15,3 +15,48 @@ inline_for_extraction noextract
 let warp_sz = 32sz
 inline_for_extraction noextract
 let warp_size = SZ.v warp_sz
+
+inline_for_extraction noextract
+val mk_kernel
+  (#et_ab #et_c : Type0)
+  {| scalar et_ab, scalar et_c |}
+  (#rows #shared #cols : szp)
+  (#lA : mlayout rows shared) {| clayout lA |}
+  (gA : gpu_matrix et_ab lA)
+  (#eA : ematrix et_ab rows shared)
+  (#lB : mlayout shared cols) {| clayout lB |}
+  (gB : gpu_matrix et_ab lB)
+  (#eB : ematrix et_ab shared cols)
+  (gC : gpu_matrix et_c (row_major rows cols))
+  (#_ : squash (SZ.fits (rows * cols)))
+  (#eC : ematrix et_c rows cols)
+  (bm : szp{bm /? rows})
+  (bn : szp{bn /? cols})
+  (bk : szp{bk /? shared})
+  (#_: squash (SZ.fits (bm * bk) /\ SZ.fits (bk * bn)))
+  (tm : szp{tm /? bm})
+  (tn : szp{tn /? bn})
+  (tk : szp{tk /? bk})
+  (wm : szp{wm * tm /? bm})
+  (wn : szp{wn * tn /? bn})
+  (#fA #fB : perm)
+  (nblk : szp{SZ.v nblk == rows/bm * (cols/bn)})
+  (nthr : szp{SZ.v nthr == bm/(wm*tm) * (bn/(wn*tn)) * warp_size})
+  (#_ : squash (SZ.fits (rows * shared)))
+  (#_ : squash (SZ.fits (rows * cols)))
+  (#_ : squash (SZ.fits (shared * cols)))
+  (#_ : squash (SZ.fits (wm * wn)))
+  (#_ : squash (SZ.fits (wm * tm)))
+  (#_ : squash (SZ.fits (wn * tn)))
+  (#_ : squash (valid_frag_et_dims et_ab FragA tm tn tk))
+  (#_ : squash (valid_frag_et_dims et_ab FragB tm tn tk))
+  (#_ : squash (valid_frag_et_dims et_c FragAcc tm tn tk))
+  (#_ : squash (valid_frag_et_comb et_ab et_c))
+  (#_ : squash (SZ.fits (bm*bk + nthr-1)))
+  (#_ : squash (SZ.fits (bk*bn + nthr-1)))
+  (#_ : squash (nblk <= max_blocks))
+  (#_ : squash (nthr <= max_threads))
+  ()
+  : kernel_desc
+      (gA |-> Frac fA eA ** gB |-> Frac fB eB ** gC |-> eC)
+      (gA |-> Frac fA eA ** gB |-> Frac fB eB ** (exists* eC'. gC |-> eC'))
